$$
\sum_{x = 2}^{4} {\frac{f(x, 2)}{{2}^{x}}} = {(\frac{f(x, 2)}{{2}^{2}})} + {(\frac{f(x, 2)}{{2}^{3}})} + {(\frac{f(x, 2)}{{2}^{4}})}
$$

$$
f(x, 2) = 1
$$

$$
\frac{1 \times }{1 \times {2}^{2}} = \frac{1}{{2}^{2}}
$$

$$
f(x, 2) = {{3 \choose 1}} - {{2 \choose 0}}
$$

$$
{3 \choose 1} = \frac{3!}{{1!} \times {2!}}
$$

$$
\frac{1 \times {2}^{1} \times {3}^{1}}{1 \times {2}^{1}} = \frac{3}{1}
$$

$$
{2 \choose 0} = \frac{2!}{{0!} \times {2!}}
$$

$$
\frac{1 \times {2}^{1}}{1 \times {2}^{1}} = \frac{1}{1}
$$

$$
{3} - {1} = 2
$$

$$
\frac{1 \times {2}^{1}}{1 \times {2}^{3}} = \frac{1}{{2}^{2}}
$$

$$
f(x, 2) = {{4 \choose 2}} - {{3 \choose 1}}
$$

$$
{4 \choose 2} = \frac{4!}{{2!} \times {2!}}
$$

$$
\frac{1 \times {2}^{1} \times {3}^{1} \times {4}^{1}}{1 \times {2}^{2}} = \frac{1 \times {2}^{1} \times {3}^{1}}{1}
$$

$$
{3 \choose 1} = \frac{3!}{{1!} \times {2!}}
$$

$$
\frac{1 \times {2}^{1} \times {3}^{1}}{1 \times {2}^{1}} = \frac{3}{1}
$$

$$
{1 \times {2}^{1} \times {3}^{1}} - {3} = 3
$$

$$
\frac{1 \times {3}^{1}}{1 \times {2}^{4}} = \frac{3}{{2}^{4}}
$$

$$
{({1} \times {{2}^{2}})} + {({{2}^{2}} \times {1})} = {(8)}
$$

$$
{({{({1} \times {{2}^{2}})} + {({{2}^{2}} \times {1})}} \times {{2}^{4}})} + {({{{2}^{2}} \times {{2}^{2}}} \times {3})} = {(176)}
$$

$$
\frac{1 \times {176}^{1}}{1 \times {2}^{8}} = \frac{11}{{2}^{4}}
$$

$$
{(\frac{f(x, 2)}{{2}^{2}})} + {(\frac{f(x, 2)}{{2}^{3}})} + {(\frac{f(x, 2)}{{2}^{4}})} = {(\frac{11}{{2}^{4}})}
$$

